mc_reify/reverse_defs.v
@@ -1,92 +1,95 @@
 Require Import floyd.proofauto.
 Require Export progs.reverse.
-(*Require Export progs.list_dt.*)
+Require Export progs.list_dt.
 Local Open Scope logic.
 
 (*Some definitions needed from the example file (verif_reverse.v) *)
-(*Instance LS: listspec t_struct_list _tail.
-Proof. eapply mk_listspec; reflexivity. Defined. *)
+Instance LS: listspec t_struct_list _tail.
+Proof. eapply mk_listspec; reflexivity. Defined. 
 
 Definition sum_int := fold_right Int.add Int.zero.
 Check var_types.
 Definition Delta : tycontext := 
 (PTree.Node
+          (PTree.Node
+             (PTree.Node
+                (PTree.Node
+                   (PTree.Node PTree.Leaf (Some (tptr t_struct_list, true))
+                      PTree.Leaf) None PTree.Leaf) None PTree.Leaf) None
+             (PTree.Node PTree.Leaf None
+                (PTree.Node PTree.Leaf (Some (tptr t_struct_list, true))
+                   PTree.Leaf))) None
+          (PTree.Node
+             (PTree.Node
+                (PTree.Node
+                   (PTree.Node PTree.Leaf (Some (tint, false)) PTree.Leaf)
+                   None PTree.Leaf) None PTree.Leaf) None
+             (PTree.Node PTree.Leaf None
+                (PTree.Node PTree.Leaf (Some (tint, true)) PTree.Leaf))),
+       PTree.empty type, tint,
+       PTree.Node
          (PTree.Node
             (PTree.Node
-               (PTree.Node
-                  (PTree.Node PTree.Leaf (Some (tptr t_struct_list, true))
-                     PTree.Leaf) None PTree.Leaf) None PTree.Leaf) None
-            (PTree.Node PTree.Leaf None
-               (PTree.Node PTree.Leaf (Some (tptr t_struct_list, true))
-                  PTree.Leaf))) None
-         (PTree.Node
+               (PTree.Node PTree.Leaf
+                  (Some
+                     (Global_func
+                        (WITH _ : unit PRE  [(1%positive, tptr tvoid),
+                         (2%positive, tptr tvoid), 
+                         (3%positive, tuint), (4%positive, tuint)]
+                         (fun _ : environ => !!False) POST  [tvoid]
+                         (fun _ : environ => !!False)))) PTree.Leaf) None
+               PTree.Leaf) None
             (PTree.Node
                (PTree.Node
-                  (PTree.Node PTree.Leaf (Some (tint, false)) PTree.Leaf)
-                  None PTree.Leaf) None PTree.Leaf) None
-            (PTree.Node PTree.Leaf None
-               (PTree.Node PTree.Leaf (Some (tint, true)) PTree.Leaf))),
-      PTree.empty _, tint, PTree.empty _).
-(*      PTree.Node
-        (PTree.Node
-           (PTree.Node
-              (PTree.Node PTree.Leaf
-                 (Some
-                    (Global_func
-                       (WITH _ : unit PRE  [(1%positive, tptr tvoid),
-                        (2%positive, tptr tvoid), (3%positive, tuint),
-                        (4%positive, tuint)](fun _ : environ => !!False)
-                        POST  [tvoid](fun _ : environ => !!False))))
-                 PTree.Leaf) None PTree.Leaf) None
-           (PTree.Node
-              (PTree.Node
-                 (PTree.Node PTree.Leaf
-                    (Some
-                       (Global_func
-                          (WITH x : share * list int PRE 
-                           [(_p, tptr t_struct_list)]
-                           (let (sh0, contents0) := x in
-                            `(lseg LS sh0 (map Vint contents0)) 
-                              (eval_id _p) `nullval) POST  [tint]
-                           (let (_, contents0) := x in
-                            local (`(eq (Vint (sum_int contents0))) retval)))))
-                    PTree.Leaf) None PTree.Leaf) None PTree.Leaf)) None
-        (PTree.Node
-           (PTree.Node
-              (PTree.Node PTree.Leaf
-                 (Some
-                    (Global_func
-                       (WITH _ : unit PRE  [(1%positive, tptr tschar),
-                        (2%positive, tint)](fun _ : environ => !!False) POST 
-                        [tint](fun _ : environ => !!False)))) PTree.Leaf)
-              None
-              (PTree.Node
-                 (PTree.Node PTree.Leaf
-                    (Some
-                       (Global_func
-                          (WITH  sh0 : share, contents0 : 
-                           list val PRE  [(_p, tptr t_struct_list)]
-                           (fun x0 : environ =>
-                            !!writable_share sh0 &&
-                            `(lseg LS sh0 contents0) (eval_id _p) `nullval x0)
-                           POST  [tptr t_struct_list]
-                           `(lseg LS sh0 (rev contents0)) retval `nullval)))
-                    PTree.Leaf)
-                 (Some (Global_var (Tarray t_struct_list 3 noattr)))
-                 PTree.Leaf)) None
-           (PTree.Node PTree.Leaf
-              (Some
-                 (Global_func
-                    (WITH _ : unit PRE  [(1%positive, tdouble)]
-                     (fun _ : environ => !!False) POST  [tdouble]
-                     (fun _ : environ => !!False))))
-              (PTree.Node
-                 (PTree.Node PTree.Leaf
-                    (Some
-                       (Global_func
-                          (WITH u : unit PRE  []main_pre prog u POST  [tint]
-                           main_post prog u))) PTree.Leaf) None PTree.Leaf)))).*)
-
+                  (PTree.Node PTree.Leaf
+                     (Some
+                        (Global_func
+                           (WITH x : share * list int PRE 
+                            [(_p, tptr t_struct_list)]
+                            (let (sh0, contents0) := x in
+                             `(lseg LS sh0 (map Vint contents0)) 
+                               (eval_id _p) `nullval) POST  [tint]
+                            (let (_, contents0) := x in
+                             local (`(eq (Vint (sum_int contents0))) retval)))))
+                     PTree.Leaf) None PTree.Leaf) None PTree.Leaf)) None
+         (PTree.Node
+            (PTree.Node
+               (PTree.Node PTree.Leaf
+                  (Some
+                     (Global_func
+                        (WITH _ : unit PRE  [(1%positive, tptr tschar),
+                         (2%positive, tint)](fun _ : environ => !!False)
+                         POST  [tint](fun _ : environ => !!False))))
+                  PTree.Leaf) None
+               (PTree.Node
+                  (PTree.Node PTree.Leaf
+                     (Some
+                        (Global_func
+                           (WITH x : share * list val PRE 
+                            [(_p, tptr t_struct_list)]
+                            (let (sh0, contents0) := x in
+                             fun x0 : environ =>
+                             !!writable_share sh0 &&
+                             `(lseg LS sh0 contents0) 
+                               (eval_id _p) `nullval x0) POST 
+                            [tptr t_struct_list]
+                            (let (sh0, contents0) := x in
+                             `(lseg LS sh0 (rev contents0)) retval `nullval))))
+                     PTree.Leaf)
+                  (Some (Global_var (Tarray t_struct_list 3 noattr)))
+                  PTree.Leaf)) None
+            (PTree.Node PTree.Leaf
+               (Some
+                  (Global_func
+                     (WITH _ : unit PRE  [(1%positive, tdouble)]
+                      (fun _ : environ => !!False) POST  [tdouble]
+                      (fun _ : environ => !!False))))
+               (PTree.Node
+                  (PTree.Node PTree.Leaf
+                     (Some
+                        (Global_func
+                           (WITH u : unit PRE  []main_pre prog u POST  [tint]
+                            main_post prog u))) PTree.Leaf) None PTree.Leaf)))).
 
 Definition Delta2 : tycontext :=
 (PTree.Node
