mc_reify/types.v
@@ -4,8 +4,10 @@ Require Import ExtLib.Core.RelDec.
 Require Import MirrorCore.TypesI.
 Require Import ExtLib.Tactics.
 Require Import ExtLib.Data.Fun.
-(*Require Import progs.list_dt. *)
+Require Import progs.list_dt. 
 Require Import Coq.FSets.FMapPositive.
+
+
 
 
 Inductive typ :=
@@ -43,13 +45,15 @@ Inductive typ :=
 | tysum : typ -> typ -> typ
 | typrod : typ -> typ -> typ
 | tyunit
-(*| tylistspec : type -> ident -> typ*)
+| tylistspec : type -> ident -> typ
 | tyOracleKind
 | tystatement
 | tyret_assert
 | tyexitkind
 | typtree : typ -> typ
 | tyglobal_spec
+| tygfield
+| tyfunspec
 (*| tyother : positive -> typ*)
 .
 
@@ -89,7 +93,7 @@ Fixpoint typD (t : typ) (*(m : PositiveMap.t Type)*): Type :=
         | tysum t1 t2 => sum (typD  t1 ) (typD  t2 )
         | typrod t1 t2 => prod (typD  t1 ) (typD  t2 )
         | tyunit => unit
-        (*| tylistspec t i => listspec t i*)  
+        | tylistspec t i => listspec t i 
         | tyOracleKind => OracleKind
         | tystatement => statement
         | tyret_assert => ret_assert
@@ -97,6 +101,8 @@ Fixpoint typD (t : typ) (*(m : PositiveMap.t Type)*): Type :=
         | tyexitkind => exitkind
         | typtree t => PTree.t (typD t)
         | tyglobal_spec => global_spec
+        | tygfield => gfield
+        | tyfunspec => funspec
     end.
 (*
 Lemma listspec_ext : forall t i (a b: listspec t i), a = b.
@@ -110,7 +116,6 @@ Qed.
 *)
 Definition typ_eq_dec : forall a b : typ, {a = b} + {a <> b}.
   decide equality.
-Defined. (*
   consider (eqb_ident i i0); intros;
   try rewrite eqb_ident_spec in H. auto.
   destruct (eqb_ident_spec i i0). right. intro. intuition. subst.
@@ -120,7 +125,7 @@ Defined. (*
   destruct (eqb_type_spec t t0).
   right; intuition; subst; congruence.
  Defined.
-*)
+
 
 Instance RelDec_eq_typ : RelDec (@eq typ) :=
 { rel_dec := fun a b =>
@@ -201,5 +206,3 @@ Instance Typ0_tyProp : Typ0 _ Prop :=
  |}.
 
 
-
- 
